theories/Labelled_Transition_System/Examples_of_LTS/SET_LTS/SetLTSConstruction.v
@@ -1,0 +1,652 @@
+(*
+   Copyright (c) 2024 Nomadic Labs
+   Copyright (c) 2024 Paul Laforgue <paul.laforgue@nomadic-labs.com>
+   Copyright (c) 2024 Léo Stefanesco <leo.stefanesco@mpi-sws.org>
+   Copyright (c) 2025 Gaëtan Lopez <glopez@irif.fr>
+
+   Permission is hereby granted, free of charge, to any person obtaining a copy
+   of this software and associated documentation files (the "Software"), to deal
+   in the Software without restriction, including without limitation the rights
+   to use, copy, modify, merge, publish, distribute, sublicense, and/or sell
+   copies of the Software, and to permit persons to whom the Software is
+   furnished to do so, subject to the following conditions:
+
+   The above copyright notice and this permission notice shall be included in all
+   copies or substantial portions of the Software.
+
+   THE SOFTWARE IS PROVIDED "AS IS", WITHOUT WARRANTY OF ANY KIND, EXPRESS OR
+   IMPLIED, INCLUDING BUT NOT LIMITED TO THE WARRANTIES OF MERCHANTABILITY,
+   FITNESS FOR A PARTICULAR PURPOSE AND NONINFRINGEMENT. IN NO EVENT SHALL THE
+   AUTHORS OR COPYRIGHT HOLDERS BE LIABLE FOR ANY CLAIM, DAMAGES OR OTHER
+   LIABILITY, WHETHER IN AN ACTION OF CONTRACT, TORT OR OTHERWISE, ARISING FROM,
+   OUT OF OR IN CONNECTION WITH THE SOFTWARE OR THE USE OR OTHER DEALINGS IN THE
+   SOFTWARE.
+*)
+
+From Coq Require ssreflect Setoid.
+From Coq.Unicode Require Import Utf8.
+From Coq.Lists Require Import List.
+Import ListNotations.
+From Coq.Wellfounded Require Import Inverse_Image.
+From Coq.Logic Require Import JMeq ProofIrrelevance.
+From Coq.Program Require Import Wf Equality.
+From stdpp Require Import base list countable decidable finite gmap gmultiset.
+From Must Require Import MultisetHelper gLts FiniteImageLTS ActTau Bisimulation.
+(* From Must Require Import MultisetHelper  Lts_OBA Lts_FW Lts_OBA_FB 
+    InListPropHelper CodePurification InteractionBetweenLts MultisetLTSConstruction ActTau. *)
+
+(**************************************** Forwarder LTS *************************************)
+
+
+Lemma exists_forall_in {B} (ps : list B) (P : B -> Prop) (Q : B -> Prop)
+  (h : forall p, p ∈ ps -> P p \/ Q p) : Exists P ps \/ Forall Q ps.
+Proof.
+  induction ps as [|p ?]. eauto.
+  destruct IHps; destruct (h p); eauto; set_solver.
+Qed.
+
+Lemma exists_forall_in_gset `{Countable A} (ps : gset A) (P : A -> Prop) (Q : A -> Prop)
+  (h : forall p, p ∈ ps -> P p \/ Q p) : (exists p, p ∈ ps /\ P p)\/ (forall p, p ∈ ps -> Q p).
+Proof.
+  induction ps using set_ind_L. set_solver.
+  destruct IHps; destruct (h x); eauto; set_solver.
+Qed.
+
+#[global] Program Instance SET_LTS `(gLtsP : @gLts P A H) `{!FiniteImagegLts P A} : @gLts (gset P) A H.
+Next Obligation.
+  intros. destruct X.
+  + exact (H1 = lts_extaction_set_from_pset H0 μ /\ H1 ≠ ∅).
+  + exact (H1 = lts_tau_set_from_pset H0 /\ H1 ≠ ∅).
+Defined.
+Next Obligation.
+  intros; simpl in *. unfold SET_LTS_obligation_1.
+  destruct α.
+  - destruct (decide (b = lts_extaction_set_from_pset a μ /\ b ≠ ∅)).
+    + left. eauto.
+    + right. eauto.
+  - destruct (decide (b = lts_tau_set_from_pset a /\ b ≠ ∅)).
+    + left. eauto.
+    + right. eauto.
+Qed.
+Next Obligation.
+  intros. exact (forall p, p ∈ H0 -> lts_refuses p X).
+Defined.
+Next Obligation.
+  intros. simpl in *. unfold SET_LTS_obligation_3.
+  destruct α.
+  - assert (forall p', p' ∈ p -> (¬ lts_refuses p' (ActExt μ) \/ lts_refuses p' (ActExt μ))) as Hyp.
+    { intros. destruct (decide (p' ↛[μ])); [right|left];eauto. }
+    (* destruct (exists_forall_in_gset p _ _ Hyp). *) admit.
+  - assert (forall p', p' ∈ p -> (¬ lts_refuses p' τ \/ lts_refuses p' τ)) as Hyp.
+    { intros. destruct (decide (p' ↛)); [right|left];eauto. }
+    (* destruct (exists_forall_in_gset p _ _ Hyp). *) admit.
+Admitted.
+Next Obligation.
+  unfold SET_LTS_obligation_3.
+  unfold SET_LTS_obligation_1. intros. destruct α.
+  - assert (forall p', p' ∈ p -> (¬ lts_refuses p' (ActExt μ) \/ lts_refuses p' (ActExt μ))) as Hyp.
+    { intros. destruct (decide (p' ↛[μ])); [right|left];eauto. }
+    exists (lts_extaction_set_from_pset p μ). split; eauto.
+    destruct (exists_forall_in_gset p _ _ Hyp).
+    + destruct H1 as (p' & Hyp' & Hyp'').
+      intro. eapply lts_refuses_spec1 in Hyp'' as (p'' & Hyp''').
+      assert (p'' ∈ lts_extaction_set_from_pset p μ).
+      { destruct (lts_extaction_set_from_pset_ispec p μ). eauto. }
+      rewrite H1 in H2. inversion H2.
+    + contradiction.
+  - assert (forall p', p' ∈ p -> (¬ lts_refuses p' τ \/ lts_refuses p' τ)) as Hyp.
+    { intros. destruct (decide (p' ↛)); [right|left];eauto. }
+    exists (lts_tau_set_from_pset p). split; eauto.
+    destruct (exists_forall_in_gset p _ _ Hyp).
+    + destruct H1 as (p' & Hyp' & Hyp'').
+      intro. eapply lts_refuses_spec1 in Hyp'' as (p'' & Hyp''').
+      assert (p'' ∈ lts_tau_set_from_pset p).
+      { destruct (lts_tau_set_from_pset_ispec p). eauto. }
+      rewrite H1 in H2. inversion H2.
+    + contradiction.
+Qed.
+Next Obligation.
+  unfold SET_LTS_obligation_3.
+  unfold SET_LTS_obligation_1. intros.
+  destruct α.
+  - intro. destruct H0 as (p' & Hyp1 & Hyp2). subst.
+    remember (lts_extaction_set_from_pset p μ).
+    induction g using set_ind_L.
+    + eapply Hyp2. reflexivity.
+    + assert (x ∈ lts_extaction_set_from_pset p μ) as Hyp by set_solver.
+      destruct (lts_extaction_set_from_pset_ispec p μ) as (Hyp'1 & Hyp'2).
+      unfold lts_extaction_set_from_pset_spec1 in Hyp'1.
+      unfold lts_extaction_set_from_pset_spec2 in Hyp'2.
+      eapply Hyp'1 in Hyp as (p'0 & in_Set & Tr).
+      eapply H1 in in_Set. eapply lts_refuses_spec2; eauto.
+  - intro. destruct H0 as (p' & Hyp1 & Hyp2). subst.
+    remember (lts_tau_set_from_pset p).
+    induction g using set_ind_L.
+    + eapply Hyp2. reflexivity.
+    + assert (x ∈ lts_tau_set_from_pset p) as Hyp by set_solver.
+      destruct (lts_tau_set_from_pset_ispec p) as (Hyp'1 & Hyp'2).
+      unfold lts_tau_set_from_pset_spec1 in Hyp'1.
+      unfold lts_tau_set_from_pset_spec2 in Hyp'2.
+      eapply Hyp'1 in Hyp as (p'0 & in_Set & Tr).
+      eapply H1 in in_Set. eapply lts_refuses_spec2 ; eauto.
+Qed.
+
+Definition set_eq `(gLtsEqP : @LtsEq P A H gLtsP) `{!FiniteImagegLts P A} (ps : gset P) (qs : gset P) :=
+  (forall p', p' ∈ ps -> exists q', q' ∈ qs /\ p' ⋍ q') /\ (forall q', q' ∈ qs -> exists p', p' ∈ ps /\ p' ⋍ q').
+
+Infix "⋍ₛₑₜ" := set_eq (at level 70).
+
+#[global] Program Instance SET_LTS_eq `(gLtsP : @gLts P A H) `{!FiniteImagegLts P A} : @gLtsEq (gset P) A H (SET_LTS gLtsP) :=
+  {| eq_rel := fw_eq |}.
+Next Obligation.
+  `{M : @gLtsObaFB P A H gLtsP gLtsEqP gLtsObaP}  
+  `{@Prop_of_Inter P (mb A) A fw_inter H gLtsP MbgLts}
+  : gLtsEq (gset P) A :=
+  {| eq_rel := fw_eq |}.
+Next Obligation. intros. split.
+  + eapply fw_eq_refl.
+  + eapply fw_eq_symm.
+  + eapply fw_eq_trans.
+Qed.
+Next Obligation.
+  intros ? ? ? ? ? ? ? ? (p, mp) (q, mq) α ((t, mt) & heq & hl).
+  eapply lts_fw_eq_spec; eauto.
+Qed.
+
+#[global] Program Instance FW_gLtsOba
+  `{M : @gLtsObaFB P A H gLtsP gLtsEqP gLtsObaP}  
+  `{@Prop_of_Inter P (mb A) A fw_inter H gLtsP MbgLts}
+  : gLtsOba (P * mb A) A :=
+  {| lts_oba_mo p := lts_oba_mo p.1 ⊎ mb_without_not_nb p.2 |}.
+Next Obligation.
+  intros ? ? ? ? ? ? ? ? p1 η p2 nb Hstep; simpl in *.
+  inversion Hstep; subst; simpl in *.
+  + apply (lts_oba_mo_spec_bis1 a1 η a2) in nb; eauto. set_solver.
+  + apply (non_blocking_action_in_ms b1 η b2) in nb as eq ; subst;  eauto. 
+    assert (η ∈ mb_without_not_nb ({[+ η +]} ⊎ b2)).
+    eapply lts_mb_nb_with_nb_spec2; eauto; try multiset_solver.
+    set_solver.
+Qed.
+Next Obligation.
+  intros ? ? ? ? ? ? ? ? (p , mem) η mem_non_blocking; simpl in *.
+  rewrite gmultiset_elem_of_disj_union in mem_non_blocking. 
+  destruct (decide (η ∈ lts_oba_mo p)) as [non_blocking_in_p | non_blocking_not_in_p].
+  + eapply lts_oba_mo_spec_bis2 in non_blocking_in_p as (p' & nb & Hstep).
+    exists (p', mem). split.
+    ++ exact nb.
+    ++ eauto with mdb.
+  + destruct (decide (η ∈ mb_without_not_nb mem)) as [non_blocking_in_mem | non_blocking_not_in_mem].
+    eapply lts_mb_nb_with_nb_spec1 in non_blocking_in_mem as (nb & mem').
+    * exists (p , mem ∖ {[+ η +]}). split.
+      ++ exact nb.
+      ++ eapply ParRight. assert (mem = {[+ η +]} ⊎ mem ∖ {[+ η +]}) as eq. multiset_solver.
+         rewrite eq at 1. eapply lts_multiset_minus. exact nb. 
+    * exfalso. destruct mem_non_blocking; contradiction.
+Qed.
+Next Obligation.
+  intros ? ? ? ? ? ? ? ? ? ? ? nb Hstep ; simpl in *.
+  inversion Hstep; subst; simpl in *.
+  - apply (lts_oba_mo_spec2 a1 η a2) in nb; eauto. multiset_solver.
+  - apply (non_blocking_action_in_ms b1 η b2) in nb as eq; eauto; subst.
+    rewrite gmultiset_disj_union_assoc. 
+    assert ({[+ η +]} ⊎ lts_oba_mo a ⊎ mb_without_not_nb b2 = 
+    lts_oba_mo a ⊎ ({[+ η +]} ⊎ mb_without_not_nb b2)) as eq. multiset_solver.
+    rewrite eq.
+    erewrite gmultiset_eq_pop_l; eauto.
+    eapply lts_mb_nb_spec1;eauto.
+Qed.
+Next Obligation.
+intros ? ? ? ? ? ? ? ? ? ? ? ? ? nb Hstep_nb Hstep. destruct p as (p, mp), q as (q, mq), r as (r, mr).
+  inversion Hstep_nb (* as [a b c d e f| a b c d e f| a b c d e f] *) ; inversion Hstep; subst.
+  - destruct (lts_oba_non_blocking_action_delay nb l l0) as (t & hlt0 & (r0 & hlr0 & heqr0)).
+    exists (t, mr). split; simpl in *. eauto with mdb.
+    exists (r0, mr). split. simpl in *. eauto with mdb.
+    now eapply fw_eq_id_mb.
+  - exists (p, mr). split; simpl in *. eauto with mdb.
+    exists (r, mr). split. simpl in *. eauto with mdb. reflexivity.
+  - destruct (lts_oba_non_blocking_action_delay nb l l1) as (t & hlt0 & (r0 & hlr0 & heqr0)).
+    exists (t, mr). split. simpl in *. eauto with mdb.
+    exists (r0, mr). split. simpl in *. eauto with mdb.
+    now eapply fw_eq_id_mb.
+  - apply (non_blocking_action_in_ms mp η mr) in nb as eq; subst; eauto.
+    exists (r, {[+ η +]} ⊎ mr).
+    split. simpl in *. eauto with mdb.
+    exists (r, mr). split. simpl in *. eauto with mdb. reflexivity.
+  - destruct α as [μ |]. 
+    + apply (non_blocking_action_in_ms mp η mq) in nb as eq; subst; eauto.
+      destruct ((decide (non_blocking μ))) as [nb' | not_nb'].
+      ++ apply (non_blocking_action_in_ms mq μ mr) in nb' as eq; subst; eauto.
+         replace ({[+ η +]} ⊎ ({[+ μ +]} ⊎ mr))
+         with ({[+ μ +]} ⊎ ({[+ η +]} ⊎ mr)) by multiset_solver.
+         exists (r, {[+ η +]} ⊎ mr). split.
+         * eapply ParRight. eapply lts_multiset_minus. exact nb'.
+         * exists (r, mr). split. eapply ParRight. eapply lts_multiset_minus. exact nb. reflexivity.
+      ++ apply (blocking_action_in_ms mq μ mr) in not_nb' as (eq & duo & nb'); subst; eauto.
+         exists (r, {[+ co μ +]} ⊎ ({[+ η +]} ⊎ mq)).
+         split.
+         * eapply ParRight. eapply lts_multiset_add; eauto.
+         * replace ({[+ co μ +]} ⊎ ({[+ η +]} ⊎ mq))
+           with ({[+ η +]} ⊎ ({[+ co μ +]} ⊎ mq)) by multiset_solver.
+           exists (r ▷ {[+ co μ +]} ⊎ mq). split. eapply ParRight. eapply lts_multiset_minus. exact nb. reflexivity.
+    + inversion l0.
+  - destruct eq as (duo & nb').
+    apply (non_blocking_action_in_ms mp η mq) in nb as eq_mem; subst; eauto.
+    apply (non_blocking_action_in_ms mq μ2 mr) in nb' as eq_mem; subst; eauto.
+    replace ({[+ η +]} ⊎ ({[+ μ2 +]} ⊎ mr))
+    with ({[+ μ2 +]} ⊎ ({[+ η +]} ⊎ mr)) by multiset_solver.
+    exists (r, ({[+ η +]} ⊎ mr)). split. eapply (ParSync μ1 μ2); eauto.
+    + split; eauto.
+    + apply lts_multiset_minus. exact nb'.
+    + exists (r ▷ mr). split. eapply ParRight. apply lts_multiset_minus; exact nb. reflexivity.
+Qed.
+Next Obligation.
+  intros ? ? ? ? ? ? ? ? ? ? ? ? ? nb not_eq Hstep_nb Hstep. 
+  destruct p as (p, mp), q1 as (q, mq), q2 as (r, mr).
+  inversion Hstep_nb; subst.
+  - inversion Hstep; subst.
+    + edestruct (lts_oba_non_blocking_action_confluence nb not_eq l l0) as (t & hlt0 & (r0 & hlr0 & heqr0)).
+      exists (t, mr). split; simpl in *. eauto with mdb.
+      exists (r0, mr). split. simpl in *. eauto with mdb.
+      now eapply fw_eq_id_mb.
+    + exists (q, mr). split. simpl in *. eauto with mdb.
+      exists (q, mr). split. simpl in *. eauto with mdb. reflexivity.
+  - inversion Hstep; subst.
+    + exists (r, mq). split; simpl in *. eauto with mdb.
+      exists (r, mq). split. simpl in *. eauto with mdb. reflexivity.
+    + eapply (non_blocking_action_in_ms mp η mq) in nb as eq; eauto ; subst.
+      destruct (decide (non_blocking μ)) as [nb' | not_nb'].
+      * eapply (non_blocking_action_in_ms ({[+ η +]} ⊎ mq) μ mr) in nb' as eq; eauto ; subst.
+        assert (neq : η ≠ μ) by naive_solver.
+        assert (μ ∈ mq) as mem. multiset_solver.
+        assert (μ ∈ {[+ η +]} ⊎ mq) as mem'. multiset_solver.
+        eapply gmultiset_disj_union_difference' in mem. rewrite mem.
+        exists (r, mq ∖ {[+ μ +]}). split.
+        ++ eapply ParRight. eapply lts_multiset_minus; eauto.
+        ++ assert (η ∈ mr) as mem''. multiset_solver. 
+           assert (mr = {[+ η +]} ⊎ (mq ∖ {[+ μ +]})) as mem'''. multiset_solver.
+           rewrite mem'''. exists (r ▷ mq ∖ {[+ μ +]}). split. 
+           eapply ParRight. eapply lts_multiset_minus; eauto. reflexivity.
+      * eapply (blocking_action_in_ms ({[+ η +]} ⊎ mq) μ mr) in not_nb' as (eq & duo & nb'); eauto ; subst.
+        exists (r ▷ {[+ co μ +]} ⊎ mq). split.
+        ++ eapply ParRight. eapply lts_multiset_add; eauto.
+        ++ assert ({[+ co μ +]} ⊎ ({[+ η +]} ⊎ mq) = {[+ η +]} ⊎ ({[+ co μ +]} ⊎ mq)) as eq. multiset_solver.
+           rewrite eq. exists (r ▷ {[+ co μ +]} ⊎ mq). split. 
+           eapply ParRight. eapply lts_multiset_minus; eauto. reflexivity.
+Qed.
+Next Obligation.
+Proof.
+  intros ? ? ? ? ? ? ? ? (p1, m1) (p2, m2) (p3, m3) η nb Hstep_nb Hstep.
+  inversion Hstep_nb ;subst.
+  - inversion Hstep ; subst.
+    + edestruct (lts_oba_non_blocking_action_tau nb l l0) as
+        [(t & hl1 & (t0 & hl0 & heq0)) | (μ & duo & t0 & hl0 & heq0)].
+      left. exists (t, m3).
+      split. simpl. eauto with mdb.
+      exists (t0, m3). split. simpl. eauto with mdb.
+      now eapply fw_eq_id_mb.
+      right. exists μ. split.  exact duo. exists (t0, m3). split. simpl. eauto with mdb.
+      now eapply fw_eq_id_mb.
+    + inversion l0.
+    + destruct eq as (duo' & nb').
+      assert (blocking μ1). eapply dual_blocks; eauto.
+      assert (neq : μ1 ≠ η). intro. subst. contradiction. 
+      edestruct (lts_oba_non_blocking_action_confluence nb neq l l1)
+        as (t & hl1 & (t1 & hl2 & heq1)).
+      left. exists (t, m3). split. eapply ParSync; eauto. split; eauto.
+      exists (t1, m3). split. simpl. eauto with mdb.
+      now eapply fw_eq_id_mb.
+  - eapply (non_blocking_action_in_ms m1 η m2) in nb as eq; subst; eauto. 
+    inversion Hstep ; subst.
+    + left. exists (p3, m2).
+      split. simpl. eauto with mdb.
+      exists (p3, m2). split. eapply ParRight; eassumption. reflexivity.
+    + inversion l0.
+    + destruct eq as (duo & nb').
+      eapply (non_blocking_action_in_ms ({[+ η +]} ⊎ m2) μ2 m3) in nb' as eq'; subst; eauto. 
+      destruct (decide (μ2 = η)) as [eq | not_eq]; subst.
+      ++ right. assert (m2 = m3) as eq_mem. multiset_solver. rewrite <-eq_mem in l2.  
+         exists μ1. split; eauto. exists (p3, m2). split. simpl. eauto with mdb. rewrite eq_mem. reflexivity.
+      ++ left. eapply (non_blocking_action_in_ms ({[+ η +]} ⊎ m2) μ2 m3) in nb' as eq; subst; eauto.
+         assert (η ∈ m3). multiset_solver.
+         assert (η ∈ {[+ μ2 +]} ⊎ m3). multiset_solver.
+         assert (μ2 ∈ m2). multiset_solver.
+         assert (μ2 ∈ {[+ η +]} ⊎ m2). multiset_solver.
+         exists (p3, m2 ∖ {[+ μ2 +]}). split. eapply (ParSync μ1 μ2); eauto.
+         split; eauto. assert (m2 = {[+ μ2 +]} ⊎ (m2 ∖ {[+ μ2 +]})) as eq_mem. multiset_solver.
+         rewrite eq_mem at 1. eapply lts_multiset_minus; eauto.
+         assert (m3 = ({[+ η +]} ⊎ (m2 ∖ {[+ μ2 +]}))) as eq_mem'. multiset_solver.
+         rewrite eq_mem'. exists (p3 ▷ m2 ∖ {[+ μ2 +]}). split.
+         eapply ParRight. eapply lts_multiset_minus; eauto. reflexivity.
+Qed.
+Next Obligation.
+  intros ? ? ? ? ? ? ? ? (p1, m1) (p2, m2) (p3, m3) η nb Hstep_nb Hstep_nb'.
+  intros p2' p3' hwp2 hwp3; simpl in *.
+  inversion Hstep_nb ; subst.
+  - inversion Hstep_nb' ; subst.
+    + eapply fw_eq_id_mb; eauto.
+      eapply lts_oba_non_blocking_action_deter; eauto.
+    + eapply (non_blocking_action_in_ms m2 η m3) in nb as eq; subst; eauto.
+      set (he1 := lts_oba_mo_spec2 _ _ _ nb l).
+      rewrite he1 in hwp3.
+      eapply strip_eq_step in hwp3 as (p0 & hw0 & heq0); eauto. split.
+      etrans. eapply strip_m_deter; eauto. eassumption.
+      assert (mb_without_not_nb ({[+ η +]} ⊎ m3) = {[+ η +]} ⊎ mb_without_not_nb m3) as eq.
+      eapply lts_mb_nb_spec1;eauto. rewrite eq.
+      rewrite he1.
+      rewrite gmultiset_disj_union_comm at 1.
+      rewrite <- 2 gmultiset_disj_union_assoc.
+      eapply gmultiset_eq_pop_l. multiset_solver.
+  - inversion Hstep_nb' ; subst.
+    + eapply (non_blocking_action_in_ms m3 η m2) in nb as eq; subst; eauto.
+      set (he1 := lts_oba_mo_spec2 _ _ _ nb l0).
+      rewrite he1 in hwp2.
+      eapply strip_eq_step in hwp2 as (p0 & hw0 & heq0); eauto. split.
+      etrans. symmetry. eassumption.
+      eapply strip_m_deter; eauto.
+      assert (mb_without_not_nb ({[+ η +]} ⊎ m2) = {[+ η +]} ⊎ mb_without_not_nb m2) as eq.
+      eapply lts_mb_nb_spec1;eauto. rewrite eq.
+      symmetry. rewrite he1.
+      rewrite gmultiset_disj_union_comm at 1.
+      rewrite <- 2 gmultiset_disj_union_assoc.
+      eapply gmultiset_eq_pop_l. multiset_solver.
+    + eapply (non_blocking_action_in_ms m1 η m2) in nb as eq; subst; eauto.
+      eapply (non_blocking_action_in_ms ({[+ η +]} ⊎ m2) η m3) in nb as eq; subst; eauto.
+      assert (m3 = m2) by multiset_solver; subst.
+      split.  eapply strip_m_deter; eauto. multiset_solver.
+Qed.
+Next Obligation.
+  intros ? ? ? ? ? ? ? ? (p1, mp1) (p2, mp2) (q1, mq1) (q2, mq2) η nb Hstep_nb Hstep_nb' equiv.
+  inversion Hstep_nb; subst;  intros p1' p2' hwp1 hwp2; simpl in *.
+  - eapply lts_oba_mo_spec2 in l as hd1; eauto.
+    edestruct (lts_oba_mo_strip q1) as (q1' & hwq1).
+    inversion Hstep_nb'; subst.
+    + edestruct (lts_oba_mo_strip q2) as (q2' & hwq2).
+      edestruct (equiv q1' q2'); eauto; simpl in *.
+      eapply lts_oba_mo_spec2 in l0 as hd2; eauto.
+      split.
+      ++ rewrite hd1 in hwp1. rewrite hd2 in hwp2.
+         eapply strip_eq_step in hwp1, hwp2; eauto.
+         destruct hwp1 as (t1 & hwq1' & heq1').
+         destruct hwp2 as (t2 & hwq2' & heq2').
+         set (heq1 := strip_m_deter hwq1 hwq1').
+         set (heq2 := strip_m_deter hwq2 hwq2').
+         transitivity t1. now symmetry.
+         transitivity q1'. now symmetry.
+         transitivity q2'. now symmetry.
+         transitivity t2. now symmetry. eassumption.
+      ++ multiset_solver.
+    + edestruct (equiv q1' p2'); eauto; simpl in *.
+      split.
+      ++ rewrite hd1 in hwp1.
+         eapply strip_eq_step in hwp1; eauto.
+         destruct hwp1 as (t1 & hwq1' & heq1').
+         set (heq1 := strip_m_deter hwq1 hwq1').
+         transitivity t1. naive_solver.
+         transitivity q1'; naive_solver.
+      ++ rewrite hd1. symmetry.
+         rewrite gmultiset_disj_union_comm at 1.
+         eapply (non_blocking_action_in_ms mp2 η mq2) in nb as eq; eauto ; subst.
+         assert (mb_without_not_nb ({[+ η +]} ⊎ mq2) = {[+ η +]} ⊎ mb_without_not_nb mq2) as eq.
+         eapply lts_mb_nb_spec1;eauto. rewrite eq.
+         rewrite <- 2 gmultiset_disj_union_assoc.
+         eapply gmultiset_eq_pop_l. multiset_solver.
+  - inversion Hstep_nb'; subst.
+    + eapply lts_oba_mo_spec2 in l0 as hd1; eauto.
+      edestruct (lts_oba_mo_strip q2) as (q2' & hwq2).
+      edestruct (equiv p1' q2'); eauto; simpl in *.
+      split.
+      ++ rewrite hd1 in hwp2.
+         eapply strip_eq_step in hwp2; eauto.
+         destruct hwp2 as (t2 & hwq2' & heq2').
+         set (heq1 := strip_m_deter hwq2 hwq2').
+         transitivity q2'. naive_solver.
+         transitivity t2; naive_solver.
+      ++ rewrite hd1.
+         rewrite gmultiset_disj_union_comm at 1.
+         eapply (non_blocking_action_in_ms mp1 η mq1) in nb as eq; eauto; subst.
+         assert (mb_without_not_nb ({[+ η +]} ⊎ mq1) = {[+ η +]} ⊎ mb_without_not_nb mq1) as eq.
+         eapply lts_mb_nb_spec1;eauto. rewrite eq.
+         rewrite <- 2 gmultiset_disj_union_assoc.
+         eapply gmultiset_eq_pop_l. multiset_solver.
+    + eapply (non_blocking_action_in_ms mp1 η mq1) in nb as eq; subst; eauto.
+      assert (mb_without_not_nb ({[+ η +]} ⊎ mq1) = {[+ η +]} ⊎ mb_without_not_nb mq1) as eq.
+      eapply lts_mb_nb_spec1;eauto. rewrite eq.
+      edestruct (equiv p1' p2'); eauto; simpl in *.
+      eapply (non_blocking_action_in_ms mp2 η mq2) in nb as eq'; subst; eauto.
+      split. assumption.
+      assert (mb_without_not_nb ({[+ η +]} ⊎ mq2) = {[+ η +]} ⊎ mb_without_not_nb mq2) as eq''.
+      eapply lts_mb_nb_spec1;eauto. rewrite eq''.
+      multiset_solver.
+Qed.
+
+(* Forwarder of a LTS with OBA axioms respects FW axioms *)
+
+#[global] Program Instance FW_gLtsObaFW
+  `{M : @gLtsObaFB P A H gLtsP gLtsEqP gLtsObaP}
+  `{@Prop_of_Inter P (mb A) A fw_inter H gLtsP MbgLts}
+  : gLtsObaFW (P * mb A) A.
+Next Obligation.
+  intros ? ? ? ? ? ? ? ? (p, m) η μ.
+  exists (p, {[+ η +]} ⊎ m). split; eauto with mdb.
+  eapply ParRight. eapply lts_multiset_add; eauto.
+  eapply ParRight. eapply lts_multiset_minus; eauto.
+Qed.
+Next Obligation.
+  intros ? ? ? ? ? ? ? ? (p1, m1) (p2, m2) (p3, m3) η μ nb duo Hstep_nb Hstep.
+  inversion Hstep_nb; subst.
+  + inversion Hstep; subst.
+    ++ left. destruct (lts_oba_fb_feedback nb duo l l0) as (t & l1 & heq).
+       exists (t, m3). split. eapply ParLeft; assumption.
+       now eapply fw_eq_id_mb.
+    ++ right. simpl. unfold fw_eq.
+       intros p' q' strip_p strip_q. simpl in *.
+       assert ( blocking μ) as not_nb. eapply dual_blocks; eauto.
+       eapply (blocking_action_in_ms m2 μ m3) in not_nb as (eq & duo' & nb'); subst.
+       set (heq := lts_oba_mo_spec2 _ _ _ nb l).
+       rewrite heq in strip_p. rewrite heq. split.
+       +++ destruct (strip_mem_ex strip_p) as (e & l' & nb'').
+           destruct (strip_eq_step strip_p e l') as (t & hwo & heq'); eauto.
+           set (h := lts_oba_non_blocking_action_deter nb'' l l').
+           etrans. symmetry. eassumption.
+           symmetry. eapply strip_eq_sim; eassumption.
+       +++ assert (mb_without_not_nb ({[+ co μ +]} ⊎ m2) 
+              = {[+ co μ +]} ⊎ mb_without_not_nb m2) as eq''.
+           eapply lts_mb_nb_spec1;eauto. rewrite eq''.
+           rewrite <- gmultiset_disj_union_assoc.
+           rewrite gmultiset_disj_union_comm.
+           rewrite <- gmultiset_disj_union_assoc.
+           eapply gmultiset_eq_pop_l.
+           assert (η = co μ) as eq_nb. eapply unique_nb; eauto; subst. subst.
+           now rewrite gmultiset_disj_union_comm.
+       +++ assumption.
+  + inversion Hstep; subst.
+    ++ left. exists (p3, m3). split. eapply ParSync; eauto. split; eauto. reflexivity.
+    ++ right. 
+       eapply (non_blocking_action_in_ms m1 η m2) in nb as eq; subst; eauto.
+       assert (blocking μ) as not_nb. eapply dual_blocks; eauto.
+       eapply (blocking_action_in_ms m2 μ m3) in not_nb as (eq & duo' & nb'); subst; eauto.
+       assert (η = co μ) as eq_nb. eapply unique_nb; eauto. subst.
+       reflexivity.
+Qed.
+
+(**********************************Forwarder Construction is a Finite Image LTS ************************)
+
+Definition lts_fw_not_non_blocking_action_set `{FiniteImagegLts P A} 
+  (p : P) (m : mb A) μ :=
+  if (decide (dual (co μ) μ /\ non_blocking (co μ))) 
+  then (p, {[+ (co μ) +]} ⊎ m) :: map (fun p => (proj1_sig p, m)) (enum $ dsig (lts_step p (ActExt $ μ)))
+  else map (fun p => (proj1_sig p, m)) (enum $ dsig (lts_step p (ActExt $ μ))).
+
+Definition lts_fw_non_blocking_action_set `{FiniteImagegLts P A} 
+  (p : P) (m : mb A) η :=
+  let ps := map (fun p => (proj1_sig p, m)) (enum $ dsig (lts_step p (ActExt $ η))) in
+  if (decide (η ∈ m)) then (p, m ∖ {[+ η +]}) :: ps else ps.
+
+
+Definition lts_fw_co_fin `{@FiniteImagegLts P A H M}
+  `{@Prop_of_Inter P (mb A) A fw_inter H M MbgLts}
+  (p : P) (η : A) (* : list (A * list P) *) :=
+  map (fun μ => (η, map proj1_sig (enum $ dsig (lts_step p (ActExt $ μ))))) 
+    (elements (lts_co_inter_action_left η p) ++ elements (lts_essential_actions_left p)).
+
+Definition lts_fw_com_fin `{@FiniteImagegLts P A H M}
+  `{@Prop_of_Inter P (mb A) A fw_inter H M MbgLts}
+  (p : P) (m : list A) : list (A * list P) :=
+  concat (map (fun η => (lts_fw_co_fin p η)) m). (* flat_map (fun η => (lts_fw_co_fin p η)) m. *)
+
+Definition lts_fw_tau_set `{@FiniteImagegLts P A H M} 
+  `{@Prop_of_Inter P (mb A) A fw_inter H M MbgLts}
+  (p : P) (m : mb A) : list (P * mb A) :=
+  let xs := map (fun p' => (proj1_sig p', m)) (enum $ dsig (fun q => p ⟶ q)) in
+  let ys :=
+    concat (map
+              (fun '(a, ps) => map (fun p => (p, m ∖ {[+ a +]})) ps)
+              (lts_fw_com_fin p (elements m) ))
+    in xs ++ ys.
+
+Lemma lts_fw_tau_set_spec1 
+  `{gLtsP : @gLts P A H}
+  `{@FiniteImagegLts P A H gLtsP} 
+  `{@Prop_of_Inter P (mb A) A fw_inter H gLtsP MbgLts}
+  p1 m1 p2 m2 :
+  (p1, m1) ⟶ (p2, m2) ->
+  (p2, m2) ∈ lts_fw_tau_set p1 m1.
+Proof.
+  intros l.
+  inversion l; subst.
+  + eapply elem_of_app. left.
+    eapply elem_of_list_fmap.
+    exists (dexist p2 l0). split. reflexivity. eapply elem_of_enum.
+  + inversion l0.
+  + assert (inter : fw_inter μ1 μ2). eauto.
+    destruct eq as (duo & nb).
+    eapply elem_of_app. right.
+    eapply elem_of_list_In.
+    eapply in_concat.
+    exists (map (fun p => (p, m2))
+         (map proj1_sig (enum $ dsig (lts_step p1 (ActExt $ μ1))))
+      ).
+    split.
+    eapply elem_of_list_In.
+    eapply elem_of_list_fmap.
+    exists (co μ1, map proj1_sig (enum $ dsig (lts_step p1 (ActExt $ μ1)))).
+    eapply (non_blocking_action_in_ms m1 μ2 m2) in nb as eq; subst; eauto.
+    assert (μ2 = co μ1) as eq. eapply unique_nb; eauto. subst.
+    split.
+    now replace (({[+ co μ1 +]} ⊎ m2) ∖ {[+ co μ1 +]}) with m2 by multiset_solver.
+    assert (elements ({[+ co μ1 +]} ⊎ m2) ≡ₚ 
+    elements (gmultiset_singleton (co μ1)) ++ elements (m2)) as equiv.
+    unfold singletonMS. eapply gmultiset_elements_disj_union.
+    assert (map (λ η : A, lts_fw_co_fin p1 η) (elements ({[+ co μ1 +]} ⊎ m2)) ≡ₚ 
+    map (λ η : A, lts_fw_co_fin p1 η) (elements ({[+(co μ1)+]} : gmultiset A) ++ elements m2))
+    as equiv2.
+    eapply Permutation_map. eauto.
+    erewrite gmultiset_elements_singleton in equiv2.
+    simpl in equiv2. 
+    assert (eq : co μ1 ▷ map proj1_sig (enum (dsig (lts_step p1 (ActExt μ1)))) ∈ 
+    lts_fw_co_fin p1 (co μ1)).
+    unfold lts_fw_co_fin.
+    edestruct (lts_essential_actions_spec_interact _ _ _ _ _ _ l1 l2 inter) 
+      as [ess_act | not_ess_act].
+    ++ rewrite map_app.  eapply elem_of_app. right. 
+       eapply elem_of_list_In. 
+       assert (lts_essential_actions_left p1 = 
+       {[μ1]} ∪ lts_essential_actions_left p1 ∖ {[μ1]}) as eq''.
+        eapply union_difference_singleton_L;eauto.
+       rewrite eq''.
+       assert (elements ({[μ1]} ∪ (lts_essential_actions_left p1) ∖ {[μ1]}) ≡ₚ
+        μ1 :: elements ((lts_essential_actions_left p1) ∖ {[μ1]})) as eq'''.
+        eapply elements_union_singleton. set_solver. symmetry in eq'''.
+       eapply Permutation_in. eapply Permutation_map. exact eq'''. simpl. left. eauto.
+    ++ assert (μ1 ∈ lts_co_inter_action_left (co μ1) p1). eauto.
+       eapply lts_co_inter_action_spec_left ; eauto.
+       rewrite map_app. 
+       eapply elem_of_app. left. 
+       eapply elem_of_list_In. 
+       assert (lts_co_inter_action_left (co μ1) p1 = 
+       {[μ1]} ∪ lts_co_inter_action_left (co μ1) p1 ∖ {[μ1]}) as eq''.
+        eapply union_difference_singleton_L;eauto.
+       rewrite eq''.
+       assert (elements ({[μ1]} ∪ (lts_co_inter_action_left (co μ1) p1) ∖ {[μ1]}) ≡ₚ
+        μ1 :: elements ((lts_co_inter_action_left (co μ1) p1) ∖ {[μ1]})) as eq'''.
+       eapply elements_union_singleton. set_solver. symmetry in eq'''.
+       eapply Permutation_in. eapply Permutation_map. exact eq'''. simpl. left. eauto.
+    ++ unfold lts_fw_com_fin. 
+    rewrite<- flat_map_concat_map.
+    assert (eq' : flat_map (λ η : A, lts_fw_co_fin p1 η) (elements ({[+ co μ1 +]} ⊎ m2))
+    ≡ₚ flat_map (λ η : A, lts_fw_co_fin p1 η) (elements ({[+ co μ1 +]} : gmultiset A) 
+      ++ (elements m2))).
+    eapply Permutation_flat_map. eauto.
+    erewrite gmultiset_elements_singleton in eq'.
+    simpl in *.
+    eapply elem_of_Permutation_proper; eauto. 
+    eapply elem_of_list_In. 
+    eapply in_or_app. left. eapply elem_of_list_In in eq. eauto.
+    ++ eapply elem_of_list_In.
+    eapply elem_of_list_fmap.
+    eexists.  split. reflexivity.
+    eapply elem_of_list_fmap.
+    exists (dexist p2 l1). split. reflexivity. eapply elem_of_enum.
+Qed.
+
+Lemma lts_fw_input_set_spec1 `{@FiniteImagegLts P A H gLtsP}
+  `{@Prop_of_Inter P (mb A) A fw_inter H gLtsP MbgLts}
+  p1 m1 p2 m2 μ :
+  (p1, m1) ⟶[μ] (p2, m2) -> blocking μ -> 
+    (p2, m2) ∈ lts_fw_not_non_blocking_action_set p1 m1 μ.
+Proof.
+  intros l not_nb.
+  inversion l; subst.
+  + unfold lts_fw_not_non_blocking_action_set.
+    destruct (decide (dual (co μ) μ /\ non_blocking (co μ))) as [(duo & nb) | case2].
+    - right. eapply elem_of_list_fmap.
+      exists (dexist p2 l0). split. reflexivity. eapply elem_of_enum.
+    - eapply elem_of_list_fmap.
+      exists (dexist p2 l0). split. reflexivity. eapply elem_of_enum.
+  + eapply (blocking_action_in_ms m1 μ m2) in not_nb as (eq & duo & nb); eauto; subst.
+    unfold lts_fw_not_non_blocking_action_set.
+    destruct (decide (dual (co μ) μ /\ non_blocking (co μ))) as [toto | impossible].
+    ++ left.
+    ++ assert (dual (co μ) μ ∧ non_blocking (co μ)); eauto. contradiction.
+Qed. 
+
+Lemma lts_fw_non_blocking_action_set_spec1 `{@FiniteImagegLts P A H gLtsP}
+  `{@Prop_of_Inter P (mb A) A fw_inter H gLtsP MbgLts}
+  p1 m1 p2 m2 η :
+  (p1, m1) ⟶[η] (p2, m2) -> non_blocking η -> 
+    (p2, m2) ∈ lts_fw_non_blocking_action_set p1 m1 η.
+Proof.
+  intros l nb.
+  inversion l; subst.
+  + unfold lts_fw_non_blocking_action_set.
+    destruct (decide (η ∈ m2)) as [in_mem | not_in_mem].
+    right. eapply elem_of_list_fmap. 
+    exists (dexist p2 l0). split. reflexivity. eapply elem_of_enum. 
+    eapply elem_of_list_fmap.
+    exists (dexist p2 l0). split. reflexivity. eapply elem_of_enum. 
+  + unfold lts_fw_non_blocking_action_set.
+    eapply (non_blocking_action_in_ms m1 η m2) in nb as eq; subst ; eauto.
+    destruct (decide (η ∈ {[+ η +]} ⊎ m2)).
+    ++ replace (({[+ η +]} ⊎ m2) ∖ {[+ η +]}) with m2 by multiset_solver.
+       left.
+    ++ multiset_solver.
+Qed.
+
+#[global] Program Instance gLtsMBFinite `{@FiniteImagegLts P A H gLtsP} 
+  `{@Prop_of_Inter P (mb A) A fw_inter H gLtsP MbgLts}
+  : FiniteImagegLts (P * mb A) A.
+Next Obligation. 
+  intros ? ? ? ? ? ? (p, m) α.
+  destruct α as [η | ].
+  + destruct (decide (non_blocking η)) as [nb | not_nb].
+    - eapply (in_list_finite (lts_fw_non_blocking_action_set p m η));
+      intros (p0, m0) h%bool_decide_unpack.
+      now eapply lts_fw_non_blocking_action_set_spec1.
+    - rename η into μ. 
+      eapply (in_list_finite (lts_fw_not_non_blocking_action_set p m μ)). simpl in *.
+      intros (p0, m0) h%bool_decide_unpack.
+      now eapply lts_fw_input_set_spec1. 
+  + eapply (in_list_finite (lts_fw_tau_set p m)).
+      intros (p0, m0) h%bool_decide_unpack.
+      now eapply lts_fw_tau_set_spec1.
+Qed.
